examples/ThreePoint.v
@@ -1,0 +1,65 @@
+Require Import StLib.Main StLib.Kernels.
+Require Import Psatz.
+
+Parameters P N : Z.
+
+Module Jacobi1D <: (PROBLEM Z2).
+  Local Open Scope aexpr.
+
+  Definition space := 〚0, N-1〛×〚0, N*P-1〛.
+  Definition target := 〚0, N-1〛×〚0, N*P-1〛.
+  Definition dep c :=
+    match c with
+      | (t,i) =>
+        [(t-1,i); (t-1,i-1); (t-1,i+1)]
+    end.
+End Jacobi1D.
+
+Module P := Kern Z2 Jacobi1D.
+Import P.
+
+Definition my_comp1 :=
+  (For "t" From 0 To N-1 Do
+     For "i" From "t" To N-"t"-1 Do
+       Fire ("t":aexpr, N*"id" + "i"))%code.
+
+Definition my_comp2 :=
+  (For "t" From 0 To N-1 Do
+     For "i" From N-"t"+1 To "t"-1 Do
+       Fire ("t":aexpr, N*"id" + "i"))%code.
+
+Definition my_comp3 :=
+  (For "t" From 0 To N-1 Do
+     For "i" From N-"t" To "t"-1 Do
+       Fire ("t":aexpr, N*"id" + "i"))%code.
+
+Definition my_comp :=
+  (If "T" =? 0 Then
+     my_comp1
+   Else
+     If "T" =? 1 Then
+       my_comp2;; my_comp3
+     Else
+       Nop)%code.
+
+Definition my_send :=
+  (If "to" =? "id" - 1 Then
+    For "t" From 0 To N-1 Do
+      Fire ("t":aexpr, N*"id" + "t")
+   Else
+     If "to" =? "id" + 1 Then
+       For "t" From 0 To N-1 Do
+         Fire ("t":aexpr, N*"id" + N-"t"-1)
+     Else
+       Nop)%code.
+
+Definition my_code :=
+  makeKernel my_comp my_send.
+
+Theorem my_code_correct :
+  kcorrect my_code (P-1) 1.
+Proof.
+  eexists; eapply trace_synth_correct; simpl.
+
+  repeat (intro || split).
+Abort.
